Update TPE proof for `<error-free> && false` reduction (#828)
Signed-off-by: John Kastner <jkastner@amazon.com>

cedar-lean/Cedar/TPE/Evaluator.lean
@@ -63,6 +63,8 @@ def and : Residual → Residual → CedarType → Residual
   | .val false _, _, _ => false
   | .error _, _, ty    => .error ty
   | l, .val true _, _  => l
+  | l, .val false rty, ty  =>
+    if l.errorFree then false else .and l (.val false rty) ty
   | l, r, ty           => .and l r ty
 
 def or : Residual → Residual → CedarType → Residual
@@ -70,6 +72,8 @@ def or : Residual → Residual → CedarType → Residual
   | .val false _, r, _ => r
   | .error _, _, ty    => .error ty
   | l, .val false _, _ => l
+  | l, .val true rty, ty  =>
+    if l.errorFree then true else .or l (.val true rty) ty
   | l, r, ty           => .or l r ty
 
 def apply₁ (op₁ : UnaryOp) (r : Residual) (ty : CedarType) : Residual :=
