cedar-lean/Cedar/Thm/TPE/ErrorFree.lean
@@ -1,0 +1,404 @@
+/-
+ Copyright Cedar Contributors
+
+ Licensed under the Apache License, Version 2.0 (the "License");
+ you may not use this file except in compliance with the License.
+ You may obtain a copy of the License at
+
+      https://www.apache.org/licenses/LICENSE-2.0
+
+ Unless required by applicable law or agreed to in writing, software
+ distributed under the License is distributed on an "AS IS" BASIS,
+ WITHOUT WARRANTIES OR CONDITIONS OF ANY KIND, either express or implied.
+ See the License for the specific language governing permissions and
+ limitations under the License.
+-/
+
+import Cedar.TPE
+import Cedar.Thm.WellTyped
+import Cedar.Thm.TPE.Input
+
+namespace Cedar.Spec
+
+inductive BinaryOp.CanError : BinaryOp → Prop where
+  | add : BinaryOp.CanError .add
+  | sub : BinaryOp.CanError .sub
+  | mul : BinaryOp.CanError .mul
+  | getTag : BinaryOp.CanError .getTag
+
+inductive UnaryOp.CanError : UnaryOp → Prop where
+  | neg : UnaryOp.CanError .neg
+
+inductive Residual.ErrorFree : Residual → Prop where
+  | val : Residual.ErrorFree (.val v ty)
+  | var : Residual.ErrorFree (.var v ty)
+  | unary : ¬ op.CanError → Residual.ErrorFree x₁ → Residual.ErrorFree (.unaryApp op x₁ ty)
+  | binary : ¬ op.CanError → Residual.ErrorFree x₁ → Residual.ErrorFree x₂ → Residual.ErrorFree (.binaryApp op x₁ x₂ ty)
+  | and : Residual.ErrorFree x₁ → Residual.ErrorFree x₂ → Residual.ErrorFree (.and x₁ x₂ ty)
+  | or : Residual.ErrorFree x₁ → Residual.ErrorFree x₂ → Residual.ErrorFree (.or x₁ x₂ ty)
+  | ite : Residual.ErrorFree x₁ → Residual.ErrorFree x₂ → Residual.ErrorFree x₃ → Residual.ErrorFree (.ite x₁ x₂ x₃ ty)
+  | hasAttr : Residual.ErrorFree x₁ → Residual.ErrorFree (.hasAttr x₁ attr ty)
+  | set : (∀ r ∈ rs, Residual.ErrorFree r) → Residual.ErrorFree (.set rs ty)
+  | record : (∀ ax ∈ axs, Residual.ErrorFree ax.snd) → Residual.ErrorFree (.record axs ty)
+
+end Cedar.Spec
+
+namespace Cedar.Thm
+
+open Cedar.Spec
+open Cedar.Validation
+
+theorem BinaryOp.can_error_spec (op : BinaryOp) : op.canError = true ↔ op.CanError := by
+  unfold BinaryOp.canError
+  split
+  case h_1 | h_2 | h_3 | h_4 =>
+    simp only [true_iff]
+    constructor
+  case h_5 =>
+    simp only [Bool.false_eq_true, false_iff]
+    intro h
+    cases h <;> contradiction
+
+theorem UnaryOp.can_error_spec (op : UnaryOp) : op.canError = true ↔ op.CanError := by
+  unfold UnaryOp.canError
+  split
+  case h_1 =>
+    simp only [true_iff]
+    constructor
+  case h_2 =>
+    simp only [Bool.false_eq_true, false_iff]
+    intro h
+    cases h
+    contradiction
+
+theorem Residual.error_free_spec (r : Residual) : r.errorFree = true ↔ r.ErrorFree := by
+  cases r
+  any_goals
+    simp only [Residual.errorFree, Bool.false_eq_true, false_iff]
+    intro hc
+    cases hc
+  case val =>
+    simp only [Residual.errorFree, true_iff]
+    constructor
+  case var =>
+    simp only [Residual.errorFree, true_iff]
+    constructor
+  case binaryApp op x₁ x₂ _ =>
+    simp only [Residual.errorFree, Bool.and_eq_true, Bool.not_eq_eq_eq_not, Bool.not_true]
+    have hop : op.canError = false ↔ ¬ op.CanError := by
+      grind [BinaryOp.can_error_spec]
+    rw [hop, error_free_spec x₁, error_free_spec x₂]
+    constructor
+    · intro ⟨⟨h₁, h₂⟩, h₃⟩
+      constructor <;> assumption
+    · intro h
+      cases h
+      and_intros <;> assumption
+  case unaryApp op x₁ _ =>
+    simp only [Residual.errorFree, Bool.and_eq_true, Bool.not_eq_eq_eq_not, Bool.not_true]
+    have hop : op.canError = false ↔ ¬ op.CanError := by
+      grind [UnaryOp.can_error_spec]
+    rw [hop, error_free_spec x₁]
+    constructor
+    · intro ⟨h₁, h₂⟩
+      constructor <;> assumption
+    · intro h
+      cases h
+      and_intros <;> assumption
+  case and x₁ x₂ _ =>
+    simp only [Residual.errorFree, Bool.and_eq_true]
+    rw [error_free_spec x₁, error_free_spec x₂]
+    constructor
+    · intro ⟨h₁, h₂⟩
+      exact .and h₁ h₂
+    · intro h
+      cases h
+      rename_i h₁ h₂
+      exact .intro h₁ h₂
+  case or x₁ x₂ _ =>
+    simp only [Residual.errorFree, Bool.and_eq_true]
+    rw [error_free_spec x₁, error_free_spec x₂]
+    constructor
+    · intro ⟨h₁, h₂⟩
+      exact .or h₁ h₂
+    · intro h
+      cases h
+      rename_i h₁ h₂
+      exact .intro h₁ h₂
+  case ite x₁ x₂ x₃ _ =>
+    simp only [Residual.errorFree, Bool.and_eq_true]
+    rw [error_free_spec x₁, error_free_spec x₂, error_free_spec x₃]
+    constructor
+    · intro ⟨⟨h₁, h₂⟩, h₃⟩
+      exact .ite h₁ h₂ h₃
+    · intro h
+      cases h
+      rename_i h₁ h₂ h₃
+      exact ⟨⟨h₁, h₂⟩, h₃⟩
+  case hasAttr x₁ _ _ =>
+    simp only [Residual.errorFree]
+    rw [error_free_spec x₁]
+    constructor
+    · intro h₁
+      exact .hasAttr h₁
+    · intro h
+      cases h
+      assumption
+  case set rs ty =>
+    simp only [Residual.errorFree, List.all_subtype, List.unattach_attach, List.all_eq_true]
+    have ih : ∀ r ∈ rs, r.errorFree = true ↔ r.ErrorFree := by
+      intro r hr
+      have : sizeOf r  < sizeOf (Residual.set rs ty) :=  by
+        have := List.sizeOf_lt_of_mem hr
+        simp only [Residual.set.sizeOf_spec, gt_iff_lt]
+        omega
+      exact error_free_spec r
+    constructor
+    · intro h
+      exact .set λ r hr => (ih r hr).mp (h r hr)
+    · intro h r hr
+      rw [ih r hr]
+      cases h
+      rename_i h
+      exact h r hr
+  case record axs ty =>
+    simp only [Residual.errorFree, List.all_eq_true, Subtype.forall, Prod.forall]
+    have ih : ∀ ax ∈ axs, ax.snd.errorFree = true ↔ ax.snd.ErrorFree := by
+      intro ax hax
+      have : sizeOf ax.snd  < sizeOf (Residual.record axs ty) :=  by
+        have := List.sizeOf_snd_lt_sizeOf_list hax
+        simp only [Residual.record.sizeOf_spec, gt_iff_lt]
+        omega
+      exact error_free_spec ax.snd
+    constructor
+    · intro h
+      constructor
+      intro ax hax
+      specialize ih ax hax
+      rw [←ih]
+      exact h ax.fst ax.snd (by simp [List.sizeOf_snd_lt_sizeOf_list hax]) (by grind [List.attach₂])
+    · intro h₁ a x hax h₂
+      replace hax : (a, x) ∈ axs := by grind [List.attach₂]
+      specialize ih (a, x) hax
+      rw [ih]
+      cases h₁
+      rename_i h₁
+      exact h₁ (a, x) (by grind [List.attach₂])
+termination_by r
+decreasing_by
+  all_goals
+    simp [*] at *
+    omega
+
+theorem error_free_evaluate_ok {r : Residual} :
+  InstanceOfWellFormedEnvironment req es env →
+  Residual.WellTyped env r →
+  r.ErrorFree →
+  (r.evaluate req es).isOk
+:= by
+  intro hwf hwt h₂
+  cases h₂
+  case val => simp [Residual.evaluate, Except.isOk_iff_exists]
+  case var =>
+    rename_i v _
+    cases v <;>
+    simp [Residual.evaluate, Except.isOk_iff_exists]
+  case unary =>
+    rename_i op _ _ _
+    simp only [Residual.evaluate]
+    rename_i x₁ _ he₁
+    cases hwt
+    rename_i hwt₁ hwt
+    have ih₁ := error_free_evaluate_ok hwf hwt₁ he₁
+    rw [Except.isOk_iff_exists] at ih₁
+    rw [ih₁.choose_spec]
+    simp only [apply₁, Except.bind_ok]
+    cases op
+    case neg =>
+      rename_i hop
+      exact False.elim (hop (by constructor))
+    case not | isEmpty | like pattern | is ty =>
+      split <;> try trivial
+      rename_i h_not_bool h_not_int h_not_set h_not_string h_not_entity
+      cases hwt
+      rename_i hty₁
+      have hty₁' := residual_well_typed_is_sound hwf hwt₁ ih₁.choose_spec
+      rw [hty₁] at hty₁'
+      first
+        | have ⟨_, h_val⟩ := instance_of_anyBool_is_bool hty₁'
+          simp [h_val] at h_not_bool
+        | have ⟨_, h_val⟩ := instance_of_set_type_is_set hty₁'
+          simp [h_val] at h_not_set
+        | have ⟨_, h_val⟩ := instance_of_string_is_string hty₁'
+          simp [h_val] at h_not_string
+        | have ⟨_, h_val⟩ := instance_of_entity_type_is_entity hty₁'
+          simp [h_val] at h_not_entity
+  case binary =>
+    rename_i op _ _ _ _
+    simp only [Residual.evaluate]
+    rw [Except.isOk_iff_exists]
+    rename_i he₁ he₂
+    cases hwt
+    rename_i hwt₁ hwt₂ hwt
+    have ih₁ := error_free_evaluate_ok hwf hwt₁ he₁
+    have ih₂ := error_free_evaluate_ok hwf hwt₂ he₂
+    rw [Except.isOk_iff_exists] at ih₁ ih₂
+    rw [ih₁.choose_spec, ih₂.choose_spec]
+    simp only [Except.bind_ok]
+    cases hwt
+    case mul | add | sub | getTag =>
+      rename_i hop _ _
+      exact False.elim (hop (by constructor))
+    case memₛ hety₁ hety₂ =>
+      have hty₁ := residual_well_typed_is_sound hwf hwt₁ ih₁.choose_spec
+      have hty₂ := residual_well_typed_is_sound hwf hwt₂ ih₂.choose_spec
+      rw [hety₁] at hty₁
+      replace ⟨_, hty₁⟩ := instance_of_entity_type_is_entity hty₁
+      rw [hety₂] at hty₂
+      replace ⟨_, hty₂, htys⟩ := instance_of_set_type_is_set hty₂
+      rw [hty₂]
+      replace ⟨hty₁, hty₁'⟩ := hty₁
+      rw [ hty₁']
+      simp only [apply₂, inₛ]
+      rename_i vs
+      cases h_euids : Data.Set.mapOrErr Value.asEntityUID vs Error.typeError
+      · have h_elem_euid : ∀ v ∈ vs, ∃ v', v.asEntityUID = .ok v' := by
+          intro v hv
+          replace ⟨_, h_ety⟩ := instance_of_entity_type_is_entity $ htys v hv
+          simp [h_ety, Value.asEntityUID]
+        unfold Data.Set.mapOrErr at h_euids
+        split at h_euids <;> try contradiction
+        rename_i h_err
+        replace ⟨x, h_err⟩ := List.mapM_error_implies_exists_error h_err
+        specialize h_elem_euid x h_err.left
+        simp [h_err.right] at h_elem_euid
+      · simp
+    case eq | eq_val | eq_entity =>
+      simp [apply₂]
+    case contains hty₁ =>
+      have hty₁' := residual_well_typed_is_sound hwf hwt₁ ih₁.choose_spec
+      rw [hty₁] at hty₁'
+      have ⟨_, h_val₁⟩ := instance_of_set_type_is_set hty₁'
+      simp [apply₂, h_val₁]
+    all_goals
+      rename_i hty₁ hty₂
+      have hty₁' := residual_well_typed_is_sound hwf hwt₁ ih₁.choose_spec
+      rw [hty₁] at hty₁'
+      first
+        | have ⟨_, h_val₁⟩ := instance_of_set_type_is_set hty₁'
+        | have ⟨_, h_val₁⟩ := instance_of_string_is_string hty₁'
+        | have ⟨_, h_val₁⟩ := instance_of_entity_type_is_entity hty₁'
+        | have ⟨_, h_val₁⟩ := instance_of_decimal_type_is_decimal hty₁'
+        | have ⟨_, h_val₁⟩ := instance_of_datetime_type_is_datetime hty₁'
+        | have ⟨_, h_val₁⟩ := instance_of_duration_type_is_duration hty₁'
+        | have ⟨_, h_val₁⟩ := instance_of_int_is_int hty₁'
+      have hty₂' := residual_well_typed_is_sound hwf hwt₂ ih₂.choose_spec
+      rw [hty₂] at hty₂'
+      first
+        | have ⟨_, h_val₂⟩ := instance_of_set_type_is_set hty₂'
+        | have ⟨_, h_val₂⟩ := instance_of_string_is_string hty₂'
+        | have ⟨_, h_val₂⟩ := instance_of_entity_type_is_entity hty₂'
+        | have ⟨_, h_val₂⟩ := instance_of_decimal_type_is_decimal hty₂'
+        | have ⟨_, h_val₂⟩ := instance_of_datetime_type_is_datetime hty₂'
+        | have ⟨_, h_val₂⟩ := instance_of_duration_type_is_duration hty₂'
+        | have ⟨_, h_val₂⟩ := instance_of_int_is_int hty₂'
+      simp [apply₂, hasTag, h_val₁, h_val₂]
+  case and | or =>
+    simp only [Residual.evaluate]
+    rw [Except.isOk_iff_exists]
+    rename_i x₁ x₂ _ he₁ he₂
+    cases hwt
+    rename_i hwt₁ hty₁ hwt₂ hty₂
+    have ih₁ := error_free_evaluate_ok hwf hwt₁ he₁
+    have ih₂ := error_free_evaluate_ok hwf hwt₂ he₂
+    rw [Except.isOk_iff_exists] at ih₁ ih₂
+    rw [ih₁.choose_spec, ih₂.choose_spec]
+    have hwts₁ := residual_well_typed_is_sound hwf hwt₁ ih₁.choose_spec
+    rw [hty₁] at hwts₁
+    have ⟨_, hb₁⟩ := instance_of_anyBool_is_bool hwts₁
+    have hwts₂ := residual_well_typed_is_sound hwf hwt₂ ih₂.choose_spec
+    rw [hty₂] at hwts₂
+    have ⟨_, hb₂⟩ := instance_of_anyBool_is_bool hwts₂
+    simp only [hb₁, hb₂, Result.as, Coe.coe, Value.asBool, Except.bind_ok]
+    split <;> simp [pure, Except.pure]
+  case ite =>
+    unfold Residual.evaluate
+    rw [Except.isOk_iff_exists]
+    rename_i x₁ x₂ x₃ _ he₁ he₂ he₃
+    cases hwt
+    rename_i hwt₁ hty₁ hwt₂ hwt₃ hty₂₃
+    have ih₁ := error_free_evaluate_ok hwf hwt₁ he₁
+    have ih₂ := error_free_evaluate_ok hwf hwt₂ he₂
+    have ih₃ := error_free_evaluate_ok hwf hwt₃ he₃
+    rw [Except.isOk_iff_exists] at ih₁ ih₂ ih₃
+    have hwts₁ := residual_well_typed_is_sound hwf hwt₁ ih₁.choose_spec
+    rw [hty₁] at hwts₁
+    replace hty₁ := instance_of_anyBool_is_bool hwts₁
+    rw [ih₁.choose_spec, hty₁.choose_spec, ih₂.choose_spec, ih₃.choose_spec]
+    cases hty₁.choose <;> simp [Value.asBool]
+  case set =>
+    simp only [Residual.evaluate]
+    rw [Except.isOk_iff_exists]
+    rename_i rs ty hrs₁
+    cases hwt
+    rename_i ty hwt _ _
+    cases hrs₂ : rs.mapM₁ fun x => x.val.evaluate req es <;>
+      simp only [Except.bind_err, Except.bind_ok, reduceCtorEq, exists_const, Except.ok.injEq, exists_eq']
+    replace ⟨_, ⟨_, hrs₂⟩⟩ := List.mapM_error_implies_exists_error hrs₂
+    rename_i r _
+    specialize hrs₁ r.val r.property
+    specialize hwt r.val r.property
+    have : sizeOf r.val  < sizeOf (Residual.set rs ty) :=  by
+      have := List.sizeOf_lt_of_mem r.property
+      simp only [Residual.set.sizeOf_spec, gt_iff_lt]
+      omega
+    have ih := error_free_evaluate_ok hwf hwt hrs₁
+    rw [Except.isOk_iff_exists] at ih
+    simp [hrs₂] at ih
+  case hasAttr =>
+    simp only [Residual.evaluate]
+    rename_i x₁ a _ he₁
+    have hwt₁ : Residual.WellTyped env x₁ := by
+      cases hwt <;> assumption
+    have ih₁ := error_free_evaluate_ok hwf hwt₁ he₁
+    rw [Except.isOk_iff_exists] at ih₁
+    rw [ih₁.choose_spec]
+    simp only [hasAttr, attrsOf, Except.bind_ok]
+    have hty₁' := residual_well_typed_is_sound hwf hwt₁ ih₁.choose_spec
+    cases hwt
+    all_goals
+      rename_i hty₁
+      rw [hty₁] at hty₁'
+      first
+        | have h_val₁ := instance_of_entity_type_is_entity hty₁'
+          rw [h_val₁.choose_spec.right]
+        | have h_val₁ := instance_of_record_type_is_record hty₁'
+          rw [h_val₁.choose_spec]
+      simp [Except.isOk, Except.toBool]
+  case record =>
+    rename_i axs ty haxs₁
+    cases hwt
+    rename_i rty hwt hrty
+    rw [Except.isOk_iff_exists]
+    simp only [Residual.evaluate]
+    cases haxs₂ : axs.mapM₂ fun x => bindAttr x.1.fst (x.1.snd.evaluate req es) <;> simp
+    replace ⟨_, ⟨_, haxs₂⟩⟩ := List.mapM_error_implies_exists_error haxs₂
+    rename_i ax hax
+    replace hax : ax.val ∈ axs := by grind [List.attach₂]
+    specialize haxs₁ ax.val hax
+    specialize hwt ax.val.fst ax.val.snd hax
+    have : sizeOf ax.val.snd < sizeOf (Residual.record axs (.record rty)) := by
+      have := List.sizeOf_snd_lt_sizeOf_list hax
+      simp only [Residual.record.sizeOf_spec, gt_iff_lt]
+      omega
+    have ih := error_free_evaluate_ok hwf hwt haxs₁
+    rw [Except.isOk_iff_exists] at ih
+    rw [ih.choose_spec] at haxs₂
+    simp [bindAttr] at haxs₂
+termination_by r
+decreasing_by
+  all_goals
+    simp [*] at *
+    omega
+
+end Cedar.Thm
